Working...

backend/LTL.v
@@ -161,6 +161,9 @@ Inductive state : Type :=
              (m: mem),                (**r memory state *)
       state.
 
+Section ORACLE.
+
+Variable fn_stack_requirements : ident -> Z.
 
 Section RELSEM.
 
@@ -242,15 +245,16 @@ Inductive step: state -> trace -> state -> Prop :=
       funsig fd = sig ->
       step (Block s f sp (Lcall sig ros :: bb) rs m)
         E0 (Callstate (Stackframe f sp rs bb :: s) fd rs m id)
-  | exec_Ltailcall: forall s f sp sig ros bb rs m fd rs' m' m'' id,
+  | exec_Ltailcall: forall s f sp sig ros bb rs m fd rs' m' m'' id m''',
       rs' = return_regs (parent_locset s) rs ->
       ros_is_ident ros rs' id ->
       find_function ros rs' = Some fd ->
       funsig fd = sig ->
       Mem.free m sp 0 f.(fn_stacksize) = Some m' ->
       Mem.return_frame m' = Some m'' ->
+      Mem.pop_stage m'' = Some m''' ->
       step (Block s f (Vptr sp Ptrofs.zero) (Ltailcall sig ros :: bb) rs m)
-        E0 (Callstate s fd rs' m'' id)
+        E0 (Callstate s fd rs' m''' id)
   | exec_Lbuiltin: forall s f sp ef args res bb rs m vargs t vres rs' m',
       eval_builtin_args ge rs sp m args vargs ->
       external_call ef ge vargs m t vres m' ->
@@ -272,17 +276,19 @@ Inductive step: state -> trace -> state -> Prop :=
       rs' = undef_regs (destroyed_by_jumptable) rs ->
       step (Block s f sp (Ljumptable arg tbl :: bb) rs m)
         E0 (State s f sp pc rs' m)
-  | exec_Lreturn: forall s f sp bb rs m m' m'',
+  | exec_Lreturn: forall s f sp bb rs m m' m'' m''',
       Mem.free m sp 0 f.(fn_stacksize) = Some m' ->
       Mem.return_frame m' = Some m'' ->
+      Mem.pop_stage m'' = Some m''' ->
       step (Block s f (Vptr sp Ptrofs.zero) (Lreturn :: bb) rs m)
-        E0 (Returnstate s (return_regs (parent_locset s) rs) m'')
-  | exec_function_internal: forall s f rs m m' sp rs' m'' id path,
+        E0 (Returnstate s (return_regs (parent_locset s) rs) m''')
+  | exec_function_internal: forall s f rs m m' sp rs' m'' id path m''',
       Mem.alloc_frame m id = (m', path) ->
       Mem.alloc m' 0 f.(fn_stacksize) = (m'', sp) ->
+      Mem.record_frame (Mem.push_stage m'') (Memory.mk_frame (fn_stack_requirements id)) = Some m''' ->
       rs' = undef_regs destroyed_at_function_entry (call_regs rs) ->
       step (Callstate s (Internal f) rs m id)
-        E0 (State s f (Vptr sp Ptrofs.zero) f.(fn_entrypoint) rs' m'')
+        E0 (State s f (Vptr sp Ptrofs.zero) f.(fn_entrypoint) rs' m''')
   | exec_function_external: forall s ef t args res rs m rs' m' id,
       args = map (fun p => Locmap.getpair p rs) (loc_arguments (ef_sig ef)) ->
       external_call ef ge args m t res m' ->
@@ -316,6 +322,9 @@ Inductive final_state: state -> int -> Prop :=
 
 Definition semantics (p: program) :=
   Semantics step (initial_state p) final_state (Genv.globalenv p).
+
+
+End ORACLE.
 
 (** * Operations over LTL *)
 
