cfrontend/Cexec.v
@@ -1886,17 +1886,19 @@ Proof.
   left. eapply imm_safe_t_callred; eauto.
 Qed.
 
+Variable fn_stack_requirements: ident -> Z.
+
 (** A state can "crash the world" if it can make an observable transition
   whose trace is not accepted by the external world. *)
 
 Definition can_crash_world (w: world) (S: state) : Prop :=
-  exists t, exists S', Csem.step ge S t S' /\ forall w', ~possible_trace w t w'.
+  exists t, exists S', Csem.step fn_stack_requirements ge S t S' /\ forall w', ~possible_trace w t w'.
 
 Theorem not_imm_safe_t:
   forall K C a m f k,
   context K RV C ->
   ~imm_safe_t K a m ->
-  Csem.step ge (ExprState f (C a) k e m) E0 Stuckstate \/ can_crash_world w (ExprState f (C a) k e m).
+  Csem.step fn_stack_requirements ge (ExprState f (C a) k e m) E0 Stuckstate \/ can_crash_world w (ExprState f (C a) k e m).
 Proof.
   intros. destruct (classic (imm_safe ge e K a m)).
   exploit imm_safe_imm_safe_t; eauto.
@@ -1973,6 +1975,8 @@ Qed.
 
 Inductive transition : Type := TR (rule: string) (t: trace) (S': state).
 
+Variable fn_stack_requirements: ident -> Z.
+
 Definition expr_final_state (f: function) (k: cont) (e: env) (C_rd: (expr -> expr) * reduction) :=
   match snd C_rd with
   | Lred rule a m => TR rule E0 (ExprState f (fst C_rd a) k e m)
@@ -2016,7 +2020,8 @@ Definition do_step (w: world) (s: state) : list transition :=
             do v' <- sem_cast v ty f.(fn_return) m;
             do m' <- Mem.free_list m (blocks_of_env ge e);
             do m'' <- Mem.return_frame m';
-            ret "step_return_2" (Returnstate v' (call_cont k) m'')
+            do m''' <- Mem.pop_stage m'';
+            ret "step_return_2" (Returnstate v' (call_cont k) m''')
         | Kswitch1 sl k =>
             do n <- sem_switch_arg v ty;
             ret "step_expr_switch" (State f (seq_of_labeled_statement (select_switch n sl)) (Kswitch2 k) e m)
@@ -2069,13 +2074,15 @@ Definition do_step (w: world) (s: state) : list transition :=
   | State f (Sreturn None) k e m =>
       do m' <- Mem.free_list m (blocks_of_env ge e);
       do m'' <- Mem.return_frame m';
-      ret "step_return_0" (Returnstate Vundef (call_cont k) m'')
+      do m''' <- Mem.pop_stage m'';
+      ret "step_return_0" (Returnstate Vundef (call_cont k) m''')
   | State f (Sreturn (Some x)) k e m =>
       ret "step_return_1" (ExprState f x (Kreturn k) e m)
   | State f Sskip ((Kstop | Kcall _ _ _ _ _) as k) e m =>
       do m' <- Mem.free_list m (blocks_of_env ge e);
       do m'' <- Mem.return_frame m';
-      ret "step_skip_call" (Returnstate Vundef k m'')
+      do m''' <- Mem.pop_stage m'';
+      ret "step_skip_call" (Returnstate Vundef k m''')
 
   | State f (Sswitch x sl) k e m =>
       ret "step_switch" (ExprState f x (Kswitch1 sl k) e m)
@@ -2096,8 +2103,9 @@ Definition do_step (w: world) (s: state) : list transition :=
       check (list_norepet_dec ident_eq (var_names (fn_params f) ++ var_names (fn_vars f)));
       let (m0,path) := Mem.alloc_frame m id in
       let (e,m1) := do_alloc_variables empty_env m0 (f.(fn_params) ++ f.(fn_vars)) in
-      do m2 <- sem_bind_parameters w e m1 f.(fn_params) vargs;
-      ret "step_internal_function" (State f f.(fn_body) k e m2)
+      do m2 <- Mem.record_frame (Mem.push_stage m1) (Memory.mk_frame (fn_stack_requirements id));
+      do m3 <- sem_bind_parameters w e m2 f.(fn_params) vargs;
+      ret "step_internal_function" (State f f.(fn_body) k e m3)
   | Callstate (External ef _ _ _) vargs k m id =>
       match do_external ef w vargs m with
       | None => nil
@@ -2128,10 +2136,11 @@ Ltac myinv :=
 
 Local Hint Extern 3 => exact I : core.
 Local Opaque Mem.alloc_frame.
+
 Theorem do_step_sound:
   forall w S rule t S',
   In (TR rule t S') (do_step w S) ->
-  Csem.step ge S t S' \/ (t = E0 /\ S' = Stuckstate /\ can_crash_world w S).
+  Csem.step fn_stack_requirements ge S t S' \/ (t = E0 /\ S' = Stuckstate /\ can_crash_world fn_stack_requirements w S).
 Proof with try (left; right; econstructor; eauto; fail).
   intros until S'. destruct S; simpl.
 (* State *)
@@ -2170,10 +2179,12 @@ Proof with try (left; right; econstructor; eauto; fail).
   (* internal *)
   destruct (Mem.alloc_frame m id) as [m0 path] eqn:?.
   destruct (do_alloc_variables empty_env m0 (fn_params f ++ fn_vars f)) as [e m1] eqn:?.
+  destruct (Mem.record_frame (Mem.push_stage m1) (mk_frame (fn_stack_requirements id))) eqn:?.
   myinv. left; right; eapply step_internal_function. eauto. eauto.
   instantiate (1:= m1).
   change e with (fst (e,m1)). change m1 with (snd (e,m1)) at 2. rewrite <- Heqp0.
-  apply do_alloc_variables_sound. eapply sem_bind_parameters_sound; eauto.
+  apply do_alloc_variables_sound. eauto. eapply sem_bind_parameters_sound; eauto.
+  myinv...
   (* external *)
   destruct p as [[[w' tr] v] m']. myinv. left; right; constructor.
   eapply do_ef_external_sound; eauto.
@@ -2198,7 +2209,7 @@ Qed.
 
 Theorem do_step_complete:
   forall w S t S' w',
-  possible_trace w t w' -> Csem.step ge S t S' -> exists rule, In (TR rule t S') (do_step w S).
+  possible_trace w t w' -> Csem.step fn_stack_requirements ge S t S' -> exists rule, In (TR rule t S') (do_step w S).
 Proof with (unfold ret; eauto with coqlib).
   intros until w'; intros PT H.
   destruct H.
@@ -2254,9 +2265,9 @@ Proof with (unfold ret; eauto with coqlib).
   rewrite H0...
   rewrite H0...
   destruct H0; subst x...
-  rewrite H0; rewrite H1...
   rewrite H0; rewrite H1; rewrite H2...
-  rewrite H1. rewrite H2. red in H0. destruct k; try contradiction...
+  rewrite H0; rewrite H1; rewrite H2; rewrite H3...
+  rewrite H1. rewrite H2. rewrite H3. red in H0. destruct k; try contradiction...
   rewrite H0...
   destruct H0; subst x...
   rewrite H0...
@@ -2265,7 +2276,8 @@ Proof with (unfold ret; eauto with coqlib).
   rewrite pred_dec_true; auto.
   rewrite H1.
   rewrite (do_alloc_variables_complete _ _ _ _ _ H2).
-  rewrite (sem_bind_parameters_complete _ _ _ _ _ _ H3)...
+  rewrite H3.
+  rewrite (sem_bind_parameters_complete _ _ _ _ _ _ H4)...
   exploit do_ef_external_complete; eauto. intro EQ; rewrite EQ. auto with coqlib.
 Qed.
 
