cfrontend/Csharpminor.v
@@ -287,6 +287,10 @@ Definition block_of_binding (id_b_sz: ident * (block * Z)) :=
 Definition blocks_of_env (e: env) : list (block * Z * Z) :=
   List.map block_of_binding (PTree.elements e).
 
+Section ORACLE.
+
+Variable fn_stack_requirements : ident -> Z.
+
 Section RELSEM.
 
 Variable ge: genv.
@@ -365,12 +369,13 @@ Inductive step: state -> trace -> state -> Prop :=
   | step_skip_block: forall f k e le m,
       step (State f Sskip (Kblock k) e le m)
         E0 (State f Sskip k e le m)
-  | step_skip_call: forall f k e le m m' m'',
+  | step_skip_call: forall f k e le m m' m'' m''',
       is_call_cont k ->
       Mem.free_list m (blocks_of_env e) = Some m' ->
       Mem.return_frame m' = Some m'' ->
+      Mem.pop_stage m'' = Some m''' ->
       step (State f Sskip k e le m)
-        E0 (Returnstate Vundef k m'')
+        E0 (Returnstate Vundef k m''')
 
   | step_set: forall f id a k e le m v,
       eval_expr e le m a v ->
@@ -433,17 +438,19 @@ Inductive step: state -> trace -> state -> Prop :=
       step (State f (Sswitch islong a cases) k e le m)
         E0 (State f (seq_of_lbl_stmt (select_switch n cases)) k e le m)
 
-  | step_return_0: forall f k e le m m' m'',
+  | step_return_0: forall f k e le m m' m'' m''',
       Mem.free_list m (blocks_of_env e) = Some m' ->
       Mem.return_frame m' = Some m'' ->
+      Mem.pop_stage m'' = Some m''' ->
       step (State f (Sreturn None) k e le m)
         E0 (Returnstate Vundef (call_cont k) m'')
-  | step_return_1: forall f a k e le m v m' m'',
+  | step_return_1: forall f a k e le m v m' m'' m''',
       eval_expr e le m a v ->
       Mem.free_list m (blocks_of_env e) = Some m' ->
       Mem.return_frame m' = Some m'' ->
+      Mem.pop_stage m'' = Some m''' ->
       step (State f (Sreturn (Some a)) k e le m)
-        E0 (Returnstate v (call_cont k) m'')
+        E0 (Returnstate v (call_cont k) m''')
   | step_label: forall f lbl s k e le m,
       step (State f (Slabel lbl s) k e le m)
         E0 (State f s k e le m)
@@ -453,15 +460,16 @@ Inductive step: state -> trace -> state -> Prop :=
       step (State f (Sgoto lbl) k e le m)
         E0 (State f s' k' e le m)
 
-  | step_internal_function: forall f vargs k m m0 m1 e le id path,
+  | step_internal_function: forall f vargs k m m0 m1 m2 e le id path,
       list_norepet (map fst f.(fn_vars)) ->
       list_norepet f.(fn_params) ->
       list_disjoint f.(fn_params) f.(fn_temps) ->
       Mem.alloc_frame m id = (m0,path) ->
       alloc_variables empty_env m0 (fn_vars f) e m1 ->
+      Mem.record_frame (Mem.push_stage m1) (Memory.mk_frame (fn_stack_requirements id )) = Some m2 ->
       bind_parameters f.(fn_params) vargs (create_undef_temps f.(fn_temps)) = Some le ->
       step (Callstate (Internal f) vargs k m id)
-        E0 (State f f.(fn_body) k e le m1)
+        E0 (State f f.(fn_body) k e le m2)
 
   | step_external_function: forall ef vargs k m t vres m' id,
       external_call ef ge vargs m t vres m' ->
@@ -498,3 +506,4 @@ Inductive final_state: state -> int -> Prop :=
 
 Definition semantics (p: program) :=
   Semantics step (initial_state p) final_state (Genv.globalenv p).
+End ORACLE.
