backend/Linearizeproof.v
@@ -32,6 +32,7 @@ Qed.
 
 Section LINEARIZATION.
 
+Variable fn_stack_requirements: ident -> Z.
 Variable prog: LTL.program.
 Variable tprog: Linear.program.
 
@@ -252,7 +253,7 @@ Lemma starts_with_correct:
   unique_labels c2 ->
   starts_with lbl c1 = true ->
   find_label lbl c2 = Some c3 ->
-  plus step tge (State s f sp c1 ls m)
+  plus (step fn_stack_requirements) tge (State s f sp c1 ls m)
              E0 (State s f sp c3 ls m).
 Proof.
   induction c1.
@@ -456,7 +457,7 @@ Lemma add_branch_correct:
   transf_function f = OK tf ->
   is_tail k tf.(fn_code) ->
   find_label lbl tf.(fn_code) = Some c ->
-  plus step tge (State s tf sp (add_branch lbl k) ls m)
+  plus (step fn_stack_requirements) tge (State s tf sp (add_branch lbl k) ls m)
              E0 (State s tf sp c ls m).
 Proof.
   intros. unfold add_branch.
@@ -554,9 +555,9 @@ Proof.
 Qed.
 
 Theorem transf_step_correct:
-  forall s1 t s2, LTL.step ge s1 t s2 ->
+  forall s1 t s2, LTL.step fn_stack_requirements ge s1 t s2 ->
   forall s1' (MS: match_states s1 s1'),
-  (exists s2', plus Linear.step tge s1' t s2' /\ match_states s2 s2')
+  (exists s2', plus (Linear.step fn_stack_requirements) tge s1' t s2' /\ match_states s2 s2')
   \/ (measure s2 < measure s1 /\ t = E0 /\ match_states s2 s1')%nat.
 Proof.
   induction 1; intros; try (inv MS).
@@ -686,7 +687,7 @@ Proof.
   (* internal functions *)
   assert (REACH: (reachable f)!!(LTL.fn_entrypoint f) = true).
     apply reachable_entrypoint.
-  monadInv H9.
+  monadInv H10.
   left; econstructor; split.
   apply plus_one. eapply exec_function_internal; eauto.
   rewrite (stacksize_preserved _ _ EQ). eauto.
@@ -729,7 +730,8 @@ Proof.
 Qed.
 
 Theorem transf_program_correct:
-  forward_simulation (LTL.semantics prog) (Linear.semantics tprog).
+  forward_simulation (LTL.semantics fn_stack_requirements prog)
+                     (Linear.semantics fn_stack_requirements tprog).
 Proof.
   eapply forward_simulation_star.
   apply senv_preserved.
