backend/Lineartyping.v
@@ -277,6 +277,7 @@ Inductive wt_state: state -> Prop :=
 
 Section SOUNDNESS.
 
+Variable fn_stack_requirements : ident -> Z.
 Variable prog: program.
 Let ge := Genv.globalenv prog.
 
@@ -298,7 +299,7 @@ Proof.
 Qed.
 
 Theorem step_type_preservation:
-  forall S1 t S2, step ge S1 t S2 -> wt_state S1 -> wt_state S2.
+  forall S1 t S2, step fn_stack_requirements ge S1 t S2 -> wt_state S1 -> wt_state S2.
 Proof.
 Local Opaque mreg_type.
   induction 1; intros WTS; inv WTS.
@@ -347,8 +348,8 @@ Local Opaque mreg_type.
   econstructor; eauto.
   eapply wt_find_function; eauto.
   apply wt_return_regs; auto. apply wt_parent_locset; auto.
-  red; simpl; intros. destruct l; simpl in *. rewrite H5; auto. destruct sl; auto; congruence.
-  red; simpl; intros. apply zero_size_arguments_tailcall_possible in H. apply H in H5. contradiction.
+  red; simpl; intros. destruct l; simpl in *. rewrite H6; auto. destruct sl; auto; congruence.
+  red; simpl; intros. apply zero_size_arguments_tailcall_possible in H. apply H in H6. contradiction.
 - (* builtin *)
   simpl in *; InvBooleans.
   econstructor; eauto.
@@ -371,7 +372,7 @@ Local Opaque mreg_type.
   simpl in *. InvBooleans.
   econstructor; eauto.
   apply wt_return_regs; auto. apply wt_parent_locset; auto.
-  red; simpl; intros. destruct l; simpl in *. rewrite H1; auto. destruct sl; auto; congruence.
+  red; simpl; intros. destruct l; simpl in *. rewrite H2; auto. destruct sl; auto; congruence.
   red; simpl; intros. auto.
 - (* internal function *)
   simpl in WTFD.
