backend/Tunnelingproof.v
@@ -260,6 +260,7 @@ End BRANCH_MAP_CORRECT.
 
 Section PRESERVATION.
 
+Variables fn_stack_requirements: ident -> Z.
 Variables prog tprog: program.
 Hypothesis TRANSL: match_prog prog tprog.
 Let ge := Genv.globalenv prog.
@@ -543,9 +544,9 @@ Proof.
 Qed.
 
 Lemma tunnel_step_correct:
-  forall st1 t st2, step ge st1 t st2 ->
+  forall st1 t st2, step fn_stack_requirements ge st1 t st2 ->
   forall st1' (MS: match_states st1 st1'),
-  (exists st2', step tge st1' t st2' /\ match_states st2 st2')
+  (exists st2', step fn_stack_requirements tge st1' t st2' /\ match_states st2 st2')
   \/ (measure st2 < measure st1 /\ t = E0 /\ match_states st2 st1')%nat.
 Proof.
   induction 1; intros; try inv MS.
@@ -553,7 +554,7 @@ Proof.
 - (* entering a block *)
   assert (DEFAULT: branch_target f pc = pc ->
     (exists st2' : state,
-     step tge (State ts (tunnel_function f) sp (branch_target f pc) tls tm) E0 st2'
+     step fn_stack_requirements tge (State ts (tunnel_function f) sp (branch_target f pc) tls tm) E0 st2'
      /\ match_states (Block s f sp bb rs m) st2')).
   { intros. rewrite H0. econstructor; split.
     econstructor. simpl. rewrite PTree.gmap1. rewrite H. simpl. eauto.
@@ -620,6 +621,7 @@ Proof.
 - (* Ltailcall *)
   exploit Mem.free_parallel_extends. eauto. eauto. intros (tm' & FREE & MEM').
   exploit Mem.return_frame_parallel_extends; eauto. intros (tm'' & RET & MEM'').
+  exploit Mem.pop_stage_extends; eauto. intros (tm''' & POP & MEM''').
   left; simpl; econstructor; split.
   eapply exec_Ltailcall with (fd := tunnel_fundef fd); eauto.
   eapply ros_is_ident_translated; eauto.
@@ -672,6 +674,7 @@ Proof.
 - (* Lreturn *)
   exploit Mem.free_parallel_extends. eauto. eauto. intros (tm' & FREE & MEM').
   exploit Mem.return_frame_parallel_extends; eauto. intros (tm'' & RET & MEM'').
+  exploit Mem.pop_stage_extends; eauto. intros (tm''' & POP & MEM''').
   left; simpl; econstructor; split.
   eapply exec_Lreturn; eauto.
   constructor; eauto using return_regs_lessdef, match_parent_locset.
@@ -679,6 +682,8 @@ Proof.
   exploit Mem.alloc_frame_extends; eauto. intros (tm' & ALLOCF & MEM').
   exploit Mem.alloc_extends. eauto. eauto. apply Z.le_refl. apply Z.le_refl.
   intros (tm'' & ALLOC & MEM'').
+  apply Mem.push_stage_extends in MEM''.
+  exploit Mem.record_frame_extends; eauto. intros (tm''' & REC & MEM''').
   left; simpl; econstructor; split.
   eapply exec_function_internal; eauto.
   simpl. econstructor; eauto using locmap_undef_regs_lessdef, call_regs_lessdef.
@@ -723,7 +728,8 @@ Proof.
 Qed.
 
 Theorem transf_program_correct:
-  forward_simulation (LTL.semantics prog) (LTL.semantics tprog).
+  forward_simulation (LTL.semantics fn_stack_requirements prog)
+                     (LTL.semantics fn_stack_requirements tprog).
 Proof.
   eapply forward_simulation_opt.
   apply senv_preserved.
