cfrontend/ClightBigstep.v
@@ -29,6 +29,10 @@ Require Import Ctypes.
 Require Import Cop.
 Require Import Clight.
 
+Section ORACLE.
+
+Variable fn_stack_requirements : ident -> Z.
+
 Section BIGSTEP.
 
 Variable ge: genv.
@@ -164,16 +168,18 @@ Inductive exec_stmt: env -> temp_env -> mem -> statement -> trace -> temp_env ->
   by the call.  *)
 
 with eval_funcall: mem -> fundef -> list val -> trace -> mem -> val -> ident -> Prop :=
-  | eval_funcall_internal: forall le m f vargs t e m0 m1 m2 m3 out vres m4 m5 id path,
+  | eval_funcall_internal: forall le m f vargs t e m0 m1 m1' m2 m3 out vres m4 m5 id path m6,
       Mem.alloc_frame m id = (m0,path) ->
       alloc_variables ge empty_env m0 (f.(fn_params) ++ f.(fn_vars)) e m1 ->
       list_norepet (var_names f.(fn_params) ++ var_names f.(fn_vars)) ->
-      bind_parameters ge e m1 f.(fn_params) vargs m2 ->
+      Mem.record_frame (Mem.push_stage m1) (Memory.mk_frame (fn_stack_requirements id)) = Some m1'->
+      bind_parameters ge e m1' f.(fn_params) vargs m2 ->
       exec_stmt e (create_undef_temps f.(fn_temps)) m2 f.(fn_body) t le m3 out ->
       outcome_result_value out f.(fn_return) vres m3 ->
       Mem.free_list m3 (blocks_of_env ge e) = Some m4 ->
       Mem.return_frame m4 = Some m5 ->
-      eval_funcall m (Internal f) vargs t m5 vres id
+      Mem.pop_stage m5 = Some m6 ->
+      eval_funcall m (Internal f) vargs t m6 vres id
   | eval_funcall_external: forall m ef targs tres cconv vargs t vres m' id,
       external_call ef ge vargs m t vres m' ->
       eval_funcall m (External ef targs tres cconv) vargs t m' vres id.
@@ -235,11 +241,12 @@ CoInductive execinf_stmt: env -> temp_env -> mem -> statement -> traceinf -> Pro
     [fd] on arguments [args] diverges, with observable trace [t]. *)
 
 with evalinf_funcall: mem -> fundef -> list val -> traceinf -> ident -> Prop :=
-  | evalinf_funcall_internal: forall m f vargs t e m0 id path m1 m2,
+  | evalinf_funcall_internal: forall m f vargs t e m0 id path m1 m1' m2,
       Mem.alloc_frame m id = (m0,path) ->
       alloc_variables ge empty_env m0 (f.(fn_params) ++ f.(fn_vars)) e m1 ->
       list_norepet (var_names f.(fn_params) ++ var_names f.(fn_vars)) ->
-      bind_parameters ge e m1 f.(fn_params) vargs m2 ->
+      Mem.record_frame (Mem.push_stage m1) (Memory.mk_frame (fn_stack_requirements id)) = Some m1'->
+      bind_parameters ge e m1' f.(fn_params) vargs m2 ->
       execinf_stmt e (create_undef_temps f.(fn_temps)) m2 f.(fn_body) t ->
       evalinf_funcall m (Internal f) vargs t id.
 
@@ -305,14 +312,14 @@ Lemma exec_stmt_eval_funcall_steps:
   (forall e le m s t le' m' out,
    exec_stmt ge e le m s t le' m' out ->
    forall f k, exists S,
-   star step1 ge (State f s k e le m) t S
+   star (step1 fn_stack_requirements) ge (State f s k e le m) t S
    /\ outcome_state_match e le' m' f k out S)
 /\
   (forall m fd args t m' res id,
    eval_funcall ge m fd args t m' res id->
    forall k,
    is_call_cont k ->
-   star step1 ge (Callstate fd args k m id) t (Returnstate res k m')).
+   star (step1 fn_stack_requirements) ge (Callstate fd args k m id) t (Returnstate res k m')).
 Proof.
   apply exec_stmt_funcall_ind; intros.
 
@@ -455,23 +462,23 @@ Proof.
   unfold S2. inv B1; simpl; econstructor; eauto.
 
 (* call internal *)
-  destruct (H4 f k) as [S1 [A1 B1]].
+  destruct (H5 f k) as [S1 [A1 B1]].
   eapply star_left. eapply step_internal_function; eauto. econstructor; eauto.
   eapply star_right. eexact A1.
-   inv B1; simpl in H4; try contradiction.
+   inv B1; simpl in H5; try contradiction.
   (* Out_normal *)
   assert (fn_return f = Tvoid /\ vres = Vundef).
     destruct (fn_return f); auto || contradiction.
-  destruct H9. subst vres. eapply step_skip_call; eauto.
+  destruct H11. subst vres. eapply step_skip_call; eauto.
   (* Out_return None *)
   assert (fn_return f = Tvoid /\ vres = Vundef).
     destruct (fn_return f); auto || contradiction.
-  destruct H10. subst vres.
-  rewrite <- (is_call_cont_call_cont k H8). rewrite <- H9.
+  destruct H12. subst vres.
+  rewrite <- (is_call_cont_call_cont k H10). rewrite <- H11.
   eapply step_return_0; eauto.
   (* Out_return Some *)
-  destruct H5.
-  rewrite <- (is_call_cont_call_cont k H8). rewrite <- H9.
+  destruct H6.
+  rewrite <- (is_call_cont_call_cont k H10). rewrite <- H11.
   eapply step_return_1; eauto.
   reflexivity. traceEq.
 
@@ -483,7 +490,7 @@ Lemma exec_stmt_steps:
    forall e le m s t le' m' out,
    exec_stmt ge e le m s t le' m' out ->
    forall f k, exists S,
-   star step1 ge (State f s k e le m) t S
+   star (step1 fn_stack_requirements) ge (State f s k e le m) t S
    /\ outcome_state_match e le' m' f k out S.
 Proof (proj1 exec_stmt_eval_funcall_steps).
 
@@ -492,7 +499,7 @@ Lemma eval_funcall_steps:
    eval_funcall ge m fd args t m' res id ->
    forall k,
    is_call_cont k ->
-   star step1 ge (Callstate fd args k m id) t (Returnstate res k m').
+   star (step1 fn_stack_requirements) ge (Callstate fd args k m id) t (Returnstate res k m').
 Proof (proj2 exec_stmt_eval_funcall_steps).
 
 Definition order (x y: unit) := False.
@@ -500,12 +507,12 @@ Definition order (x y: unit) := False.
 Lemma evalinf_funcall_forever:
   forall m fd args T k id,
   evalinf_funcall ge m fd args T id ->
-  forever_N step1 order ge tt (Callstate fd args k m id) T.
+  forever_N (step1 fn_stack_requirements) order ge tt (Callstate fd args k m id) T.
 Proof.
   cofix CIH_FUN.
   assert (forall e le m s T f k,
           execinf_stmt ge e le m s T ->
-          forever_N step1 order ge tt (State f s k e le m) T).
+          forever_N (step1 fn_stack_requirements) order ge tt (State f s k e le m) T).
   cofix CIH_STMT.
   intros. inv H.
 
@@ -570,7 +577,7 @@ Proof.
 Qed.
 
 Theorem bigstep_semantics_sound:
-  bigstep_sound (bigstep_semantics prog) (semantics1 prog).
+  bigstep_sound (bigstep_semantics prog) (semantics1 fn_stack_requirements prog).
 Proof.
   constructor; simpl; intros.
 (* termination *)
@@ -587,3 +594,5 @@ Proof.
 Qed.
 
 End BIGSTEP_TO_TRANSITIONS.
+
+End ORACLE.
