x86/Asm.v
@@ -942,19 +942,24 @@ Definition exec_instr (f: function) (i: instruction) (rs: regset) (m: mem) : out
       Next (nextinstr rs) m
   | Pallocframe sz ofs_ra ofs_link =>
     match rs # PC with
-      |Vptr (Global id) _  =>
-      let (m0,path) := Mem.alloc_frame m id in
-      let (m1, stk) := Mem.alloc m0 0 sz in
+    |Vptr (Global id) _
+     =>
+     let (m0,path) := Mem.alloc_frame m id in
+     let (m1, stk) := Mem.alloc m0 0 sz in
+     match Mem.record_frame (Mem.push_stage m1) (Memory.mk_frame sz) with
+     |None => Stuck
+     |Some m2 =>
       let sp := Vptr stk Ptrofs.zero in
-      match Mem.storev Mptr m1 (Val.offset_ptr sp ofs_link) rs#RSP with
+      match Mem.storev Mptr m2 (Val.offset_ptr sp ofs_link) rs#RSP with
       | None => Stuck
-      | Some m2 =>
-          match Mem.storev Mptr m2 (Val.offset_ptr sp ofs_ra) rs#RA with
-          | None => Stuck
-          | Some m3 => Next (nextinstr (rs #RAX <- (rs#RSP) #RSP <- sp)) m3
-          end
+      | Some m3 =>
+        match Mem.storev Mptr m3 (Val.offset_ptr sp ofs_ra) rs#RA with
+        | None => Stuck
+        | Some m4 => Next (nextinstr (rs #RAX <- (rs#RSP) #RSP <- sp)) m4
+        end
       end
-      |_ => Stuck
+     end
+    |_ => Stuck
     end
   | Pfreeframe sz ofs_ra ofs_link =>
       match Mem.loadv Mptr m (Val.offset_ptr rs#RSP ofs_ra) with
@@ -967,11 +972,16 @@ Definition exec_instr (f: function) (i: instruction) (rs: regset) (m: mem) : out
               | Vptr stk ofs =>
                   match Mem.free m stk 0 sz with
                   | None => Stuck
-                  | Some m' => match Mem.return_frame m' with
-                               | None => Stuck
-                               | Some m'' =>
-                                 Next (nextinstr (rs#RSP <- sp #RA <- ra)) m''
-                              end
+                  | Some m' =>
+                    match Mem.return_frame m' with
+                    | None => Stuck
+                    | Some m'' =>
+                      match Mem.pop_stage m'' with
+                        | None => Stuck
+                        | Some m''' =>
+                        Next (nextinstr (rs#RSP <- sp #RA <- ra)) m'''
+                      end
+                    end
                   end
               | _ => Stuck
               end
